added block sizes and updates proofs, block size probably should not be hidden also we need to update is_valid_loc and or add is_begin

misc-verification/slab_allocator.v
@@ -10,35 +10,34 @@ Definition freelist_push : val := λ: "fl" "l",
   "l" <- !"fl" ;; 
   "fl" <- SOME "l".
 
-(*TODO(Ben): first hide res, gets block size, store it*)
-Definition new_alloc_lazy : val := λ: "n", 
-  let: "lbase" := AllocN ("n" + #3) NONE in 
-  "lbase" <- NONE ;;
-  "lbase" +ₗ #1 <- "n" ;;
-  "lbase" +ₗ #2 <- #0 ;;
-  "lbase".
+Definition new_alloc_lazy : val := λ: "n" "bs", 
+  let: "al" := AllocN ("n" * "bs" + #4) NONE in 
+  "al" <- NONE ;;
+  "al" +ₗ #1 <- "n" ;;
+  "al" +ₗ #2 <- #0 ;;
+  "al" +ₗ #3 <- "bs" ;;
+  "al".
 
 Definition free : val := λ: "al" "l", freelist_push "al" "l".
 
-(*TODO(Ben): takes block size and does c * bz*)
-Definition freelist_extend : val := rec: "rec" "fl" "lb" "n" "c" :=
+Definition freelist_extend : val := rec: "rec" "fl" "lb" "bs" "n" "c" :=
   if: "c" + #1 ≤ "n"
-  then freelist_push "fl" ("lb" +ₗ "c") ;;
-       "rec" "fl" "lb" "n" ("c" + #1)
+  then freelist_push "fl" ("lb" +ₗ ("c" * "bs")) ;;
+       "rec" "fl" "lb" "bs" "n" ("c" + #1)
   else #().
   
-(*TODO(Ben): takes block size and does (cap + ext - 1) * bz and base is + bz * cap*)
 Definition extend : val := λ: "al", 
   let: "fl" := "al" in
   let: "res" := !("al" +ₗ #1) in 
   let: "cap" := !("al" +ₗ #2) in 
+  let: "bs" := !("al" +ₗ #3) in
   let: "mext" := if: "cap" = #0 then #1 else "cap" in
   let: "ext" := if: "mext" ≤ "res" - "cap" then "mext" else "res" - "cap" in 
   if: "ext" = #0 then NONE 
   else 
-    freelist_extend "fl" ("al" +ₗ (#3 + "cap")) ("ext" - #1) #0 ;;
+  freelist_extend "fl" ("al" +ₗ (#4 + "cap" * "bs")) "bs" ("ext" - #1) #0 ;;
     ("al" +ₗ #2) <- ("cap" + "ext") ;;
-    SOME ("al" +ₗ (#3 + "cap" + "ext" - #1)).
+    SOME ("al" +ₗ (#4 + ("cap" + "ext" - #1) * "bs")).
 
 Definition alloc : val := λ: "al", 
   match: freelist_pop "al" with 
@@ -50,241 +49,282 @@ Section Hoare.
   Context `{!heapGS_gen hlc Σ}.
 
   Implicit Types l lbase al fl : loc.
-  Implicit Types n i res cap size : nat.
+  Implicit Types n i res cap size bs : nat.
   Implicit Types v w : val.
-
+  
+  (*TODO: 
+    free function should check bounds of pointer i think or only proof? but how
+     free also now exposes internal details
+  *)
+  (*TODO: maybe make multiple of bs in is valid? or is begin seperately?*)
+  (*TODO: ask how to solve a bunch of 'lia' goals without having to split each time*)
+  (*TOOD: can we hide bs somehow, now we get uggly lemmas*)
   Definition is_valid_loc l al : iProp Σ := 
-    ∃ res (i : nat), (al +ₗ 1) ↦□ #res ∗ ⌜l = (al +ₗ (3 + i))⌝ ∗ ⌜i < res⌝.
+    ∃ (res bs i : nat), (al +ₗ 1) ↦□ #res ∗ (al +ₗ 3) ↦□ #bs ∗ 
+      ⌜l = (al +ₗ (4 + i * bs))⌝ ∗ ⌜i < res⌝.
 
   Global Instance is_valid_loc_presist l al : Persistent (is_valid_loc l al).
   Proof. apply _. Qed.
 
   Fixpoint is_freelist_rec l al size : iProp Σ := 
+    ∃ bs, (al +ₗ 3) ↦□  #(S bs) ∗
     match size with 
-    | O => l ↦ NONEV ∗ is_valid_loc l al 
-    | S s => ∃ l1, l ↦ SOMEV #l1 ∗ is_valid_loc l al ∗ is_freelist_rec l1 al s
+    | O => l ↦ NONEV ∗ ([∗ list] i ∈ seq 1 bs, ∃ v, (l +ₗ i) ↦  v) ∗ is_valid_loc l al 
+    | S s => ∃ l1, l ↦ SOMEV #l1 ∗ ([∗ list] i ∈ seq 1 bs, ∃ v, (l +ₗ i) ↦  v) ∗
+          is_valid_loc l al ∗ is_freelist_rec l1 al s
     end.
     
-  Definition is_freelist l al : iProp Σ := 
-    l ↦ NONEV 
+  Definition is_freelist al : iProp Σ := 
+    al ↦ NONEV 
       ∨
-    ∃ l1 size, l ↦ SOMEV #l1 ∗ is_freelist_rec l1 al size.
+    ∃ l1 size, al ↦ SOMEV #l1 ∗ is_freelist_rec l1 al size.
 
-  (*res now has fractional ownership and is only readable (box) 
-    now we can hide it, now can also never free l +ₗ 1*)
   Definition is_allocator (al : loc) : iProp Σ := 
-    ∃ res cap vs, ⌜res > 0⌝ ∗ ⌜cap ≤ res⌝ ∗ (al +ₗ 1) ↦□  #res ∗ 
-      (al +ₗ 2) ↦ #cap ∗ is_freelist al al ∗  
-      (al +ₗ (3 + cap)) ↦∗ vs ∗ ⌜length vs = res - cap⌝.
+    ∃ (res bs cap : nat), ⌜res > 0⌝ ∗ ⌜cap ≤ res⌝ ∗ ⌜bs > 0⌝ ∗ (al +ₗ 1) ↦□  #res ∗ 
+      (al +ₗ 2) ↦ #cap ∗ (al +ₗ 3) ↦□  #bs ∗ is_freelist al ∗  
+      (al +ₗ (4 + cap * bs)) ↦∗ replicate ((res - cap) * bs) NONEV. 
 
-  Lemma new_alloc_hoare res : 
-    {{{ ⌜res > 0⌝ }}} 
-      new_alloc_lazy #res 
+  Lemma new_alloc_hoare res bs : 
+    {{{ ⌜res > 0⌝ ∗ ⌜bs > 0⌝ }}} 
+      new_alloc_lazy #res #bs 
     {{{ al, RET #al; is_allocator al }}}.
   Proof. 
-    iIntros (φ) "%Hn Hphi". iUnfold new_alloc_lazy. wp_pures.
+    iIntros (φ) "(%Hn & %Hbs) Hphi". iUnfold new_alloc_lazy. wp_pures.
     wp_apply wp_allocN; [lia|done|]. iIntros "%al (HalN & _)". 
-    assert (Heq : Z.to_nat (res + 3) = S (S (S (Z.to_nat res)))) by lia.
-    rewrite Heq. simpl. rewrite 3!array_cons.
-    iDestruct "HalN" as "(Hal & Hal1 & Hal2 & HalN)". wp_store. wp_store. 
-    rewrite 2!Loc.add_assoc. wp_store. iApply "Hphi". 
-    iExists res, 0. iMod (pointsto_persist with "Hal1") as "#Hal1". iFrame.
-    iSplitR; [by iPureIntro|]. iSplitR; [iPureIntro; lia|]. iSplitR; [done|].
-    iPureIntro. rewrite length_replicate. lia.
+    assert (Heq : Z.to_nat (res * bs + 4) = S (S (S (S (res * bs))))) by lia.
+    rewrite Heq. simpl. rewrite 4!array_cons.
+    iDestruct "HalN" as "(Hal & Hal1 & Hal2 & Hal3 & HalN)". wp_store. wp_store.
+    rewrite 3!Loc.add_assoc. wp_store. wp_store. iApply "Hphi". 
+    iExists res, bs, 0. 
+    iMod (pointsto_persist with "Hal1") as "#Hal1". 
+    iMod (pointsto_persist with "Hal3") as "#Hal3". iFrame "Hal Hal1 Hal2 Hal3".
+    iSplitR; [by iPureIntro|]. iSplitR; [iPureIntro; lia|]. iSplitR; [by iPureIntro|]. 
+    by rewrite Z.mul_0_l Nat.sub_0_r.
   Qed.
 
-   Lemma freelist_pop_hoare fl al : 
-    {{{ is_freelist fl al }}} 
-      freelist_pop #fl
+  Lemma freelist_pop_hoare al bs : 
+    {{{ (al +ₗ 3) ↦□ #bs ∗ is_freelist al }}} 
+      freelist_pop #al
     {{{ vret, RET vret; 
-      is_freelist fl al ∗
+      is_freelist al ∗
       (⌜vret = NONEV⌝ 
         ∨ 
-      ∃ l v, ⌜vret = SOMEV #l⌝ ∗ l ↦ v ∗ is_valid_loc l al)
+      ∃ l, ⌜vret = SOMEV #l⌝ ∗ 
+        ([∗ list] i ∈ seq 0 bs, ∃ v, (l +ₗ i) ↦ v) ∗ is_valid_loc l al)
     }}}. 
   Proof.
-    iIntros (φ) "[Hl | (%l1 & %s & Hl & Hflr)] Hphi"; 
+    iIntros (φ) "(#Hal3 & [H | (%l1 & %s & Hfl & Hflr)]) Hphi"; 
     iUnfold freelist_pop; wp_load; wp_pures.
     { iApply "Hphi". iFrame. by iLeft. }
     destruct s; simpl.
-    { iDestruct "Hflr" as "(Hl1 & Hvl)". wp_load. wp_store. wp_pures. 
-      iApply "Hphi". iFrame. iRight. by iFrame. }
-    iDestruct "Hflr" as "(%l0 & Hl1 & Hl1v & Hflr)". wp_load. wp_store.
-    wp_pures. iApply "Hphi". iSplitR "Hl1 Hl1v"; [iRight; by iFrame|].
-    iRight. by iFrame.   
+    { iDestruct "Hflr" as "(%bs1 & #Hal3' & Hl1 & Hl1r & #Hl1v)". 
+      wp_load. wp_store. wp_pures. iApply "Hphi". iFrame. iRight. 
+      iExists l1. iFrame. iSplitR; [by iPureIntro|].
+      iCombine "Hal3 Hal3'" gives %[_ Heq]. simplify_eq. simpl. iFrame "Hl1v Hl1r". 
+      iExists NONEV. by rewrite Loc.add_0. }
+    iDestruct "Hflr" as "(%bs1 & #Hal3' & %l & Hl1 & Hl1r & #Hl1v & Hflr)". 
+    wp_load. wp_store. wp_pures. iApply "Hphi". 
+    iSplitL "Hfl Hflr"; [iRight; by iFrame|]. iRight.     
+    iCombine "Hal3 Hal3'" gives %[_ Heq]. simplify_eq. simpl. iFrame "Hl1v Hl1r". 
+    iSplitR; [by iPureIntro|]. rewrite Loc.add_0. auto. 
   Qed.
 
-  Lemma freelist_push_hoare l fl al : 
-    {{{ is_freelist fl al ∗ (∃ v, l ↦ v) ∗ is_valid_loc l al }}}
-      freelist_push #fl #l
-    {{{ RET #(); is_freelist fl al }}}.
+  Lemma freelist_push_hoare l al : 
+    {{{ 
+      ∃ bs, (al +ₗ 3) ↦□ #(S bs) ∗
+      is_freelist al ∗ (([∗ list] i ∈ seq 0 (S bs), ∃ v, (l +ₗ i) ↦ v)) ∗ 
+      is_valid_loc l al 
+    }}}
+      freelist_push #al #l
+    {{{ RET #(); is_freelist al }}}.
   Proof. 
-    iIntros (φ) "([Hfl|(%l1&%s&Hfl&Hisfl)]&(%v&Hl)&Hlv) Hphi"; 
-    iUnfold freelist_push; wp_load; wp_store; wp_store.
-    { iApply "Hphi". iRight. iFrame. iExists 0. by iFrame. }
+    simpl. rewrite Loc.add_0. iIntros (φ) "(%bs&#Hal3&[H | (%l1 & %s & Hfl & Hflr)] & 
+    ((%v & Hl) & Hl1bs) & Hlv) Hphi"; iUnfold freelist_push; wp_load; wp_store; 
+    wp_store. { iApply "Hphi". iRight. iFrame. iExists 0. iFrame. by iFrame "Hal3". }
     iApply "Hphi". iRight. iExists l, (S s). by iFrame. 
   Qed.
 
-  (*shouldn't we have a problem here? 
-     since we own a lot of locations that are valid locations 
-     it is possible that l is one of those locations and then 
-     we should derive a contradiciton..
-     but from alloc you always get an is_valid_loc that is 
-     also within cap so it should not be an issue *)
   Lemma free_hoare l al : 
-    {{{ is_allocator al ∗ (∃ v, l ↦ v) ∗ is_valid_loc l al }}}
+    {{{
+      ∃ bs, (al +ₗ 3) ↦□ #(S bs) ∗ (*TODO(Ben): but now use sees this?*)
+      is_allocator al ∗ (([∗ list] i ∈ seq 0 (S bs), ∃ v, (l +ₗ i) ↦ v)) ∗ 
+      is_valid_loc l al 
+    }}}
       free #al #l
     {{{ RET #(); is_allocator al }}}.
   Proof.
-    iIntros (φ) "((%res&%cap&%vs&%Hr&%Hcr&Hal1&Hal2&Hfl&Hun) & (%v & Hl) & #Hlv) Hphi".
-    iUnfold free. wp_pures. iApply (freelist_push_hoare with "[Hfl Hl]"); [by iFrame|].
-    iNext. iIntros "Hfl". iApply "Hphi". iFrame. auto.
+    iIntros (φ) "(%bs'&#Hal3'&(%res&%bs&%cap&%Hr&%Hcr&%Hbs&#Hal1&Hal2&#Hal3&Hfl&Hun)
+    &Hlbs&#Hlv) Hphi". iUnfold free. wp_pures. 
+    iApply (freelist_push_hoare with "[Hfl Hlbs]").
+    - iFrame. iFrame "Hlv Hal3'".
+    - iNext. iIntros "Hfl". iApply "Hphi". iFrame. auto.
   Qed.
 
-  Lemma freelist_extend_hoare fl al res lb cap n c d : 
+  Lemma seq_array_pointsto_eq l dq v n :
+    l ↦∗{dq} replicate n v ⊣⊢
+    ([∗ list] i ∈ seq 0 n, (l +ₗ (i : nat)) ↦{dq} v).
+  Proof.
+    iIntros. iSplit;
+    rewrite /array; iInduction n as [|n' IH] forall (l); simpl; [done| |done|];
+    iIntros "[$ Hl]"; rewrite -fmap_S_seq big_sepL_fmap;
+    setoid_rewrite Nat2Z.inj_succ; setoid_rewrite <-Z.add_1_l;
+    setoid_rewrite <-Loc.add_assoc; iApply "IH"; done.
+  Qed.
+
+  Lemma freelist_extend_hoare al res bs lb cap n c d : 
     d = n - c -> 
-    lb = (al +ₗ (3 + cap)) ->
+    lb = (al +ₗ (4 + cap * bs)) ->
     cap ≤ res ->
     n ≤ res - cap ->
+    bs > 0 ->
     {{{ 
-      (al +ₗ 1) ↦□ #res ∗ 
-      is_freelist fl al ∗ ∃ vs, (lb +ₗ c) ↦∗ vs ∗ ⌜length vs = d⌝ 
+      (al +ₗ 1) ↦□ #res ∗ (al +ₗ 3) ↦□ #bs ∗
+      is_freelist al ∗ (lb +ₗ (c * bs)) ↦∗ replicate (d * bs) NONEV 
     }}} 
-      freelist_extend #fl #lb #n #c
-    {{{ RET #(); is_freelist fl al }}}. 
+      freelist_extend #al #lb #bs #n #c
+    {{{ RET #(); is_freelist al }}}. 
   Proof. 
     iInduction d as [|d IH] forall (c); simpl; 
-    iIntros (Hd -> Hcr Hd2 φ) "(#Hal1 & Hisfl & %vs & Hun & %Hlen) Hphi"; 
+    iIntros (Hd -> Hcr Hd2 Hbs φ) "(#Hal1 & #Hal3 & Hfl & Hun) Hphi"; 
     iUnfold freelist_extend; wp_pures. 
     { case_bool_decide; [lia|]. wp_pures. by iApply "Hphi". }
-    case_bool_decide; [|lia]. wp_pures. destruct vs;
-    [rewrite length_nil in Hlen; lia|]. rewrite array_cons.
-    iDestruct "Hun" as "(Hun1 & Hun)". 
-    wp_apply (freelist_push_hoare with "[Hisfl Hun1]").
-    { iFrame. iExists res, (cap + c). iFrame "Hal1". rewrite Loc.add_assoc. 
-      iPureIntro. split; [|lia]. by rewrite Nat2Z.inj_add Z.add_assoc. }
-    iIntros "Hisfl". wp_pure. wp_pure. wp_pure. fold freelist_extend.  
+    case_bool_decide; [|lia]. wp_pures. 
+    rewrite replicate_add array_app length_replicate. 
+    iDestruct "Hun" as "(Hun1 & Hun2)". 
+    wp_apply (freelist_push_hoare with "[Hfl Hun1]").
+    { iFrame "Hfl". iExists (bs - 1). assert (S (bs - 1) = bs) by lia. rewrite H0.
+      iFrame "Hal3 Hal1". iSplitL "Hun1". 
+      - Search "↦∗" replicate. iApply big_sepL_mono; 
+        [|iApply seq_array_pointsto_eq; iApply "Hun1"]. iIntros. auto.
+      - iExists (cap + c). iPureIntro. split; [|lia]. rewrite Loc.add_assoc. 
+        f_equal. lia. }
+    iIntros "Hfl". wp_pure. wp_pure. wp_pure. fold freelist_extend.  
     assert (Heq : (Z.of_nat c + 1)%Z = Z.of_nat (c + 1)) by lia. rewrite Heq. 
-    iApply ("IH" with "[] [] [] [] [Hisfl Hun]"); 
-    try iPureIntro; [lia|done|lia|lia| |]. 
-    { iFrame "Hal1". iSplitR "Hun"; [done|]. iExists vs. iSplitL; 
-      [by rewrite Loc.add_assoc Nat2Z.inj_add|]. iPureIntro. simpl in Hlen. lia. }
-    iNext. iIntros "Hfl". by iApply "Hphi".  
+    iApply ("IH" with "[] [] [] [] [] [Hfl Hun2]"); try iPureIntro; 
+    [lia|done|lia|lia|done| |]. 
+    { iFrame "Hal1 Hal3 Hfl". rewrite Loc.add_assoc. 
+      by rewrite Nat2Z.inj_add Z.mul_add_distr_r Z.mul_1_l. }
+    iNext. iIntros. by iApply "Hphi".
   Qed. 
 
-  Lemma extend_hoare al : 
-    {{{ is_allocator al }}} 
+  Lemma extend_hoare al bs : 
+    {{{ (al +ₗ 3) ↦□ #bs ∗ is_allocator al }}} 
       extend #al 
       {{{ vret, RET vret; 
         is_allocator al ∗ 
-        ((∃ l v, ⌜vret = SOMEV #l⌝ ∗ l ↦ v ∗ is_valid_loc l al) 
+        ((∃ l, ⌜vret = SOMEV #l⌝ ∗ (([∗ list] i ∈ seq 0 bs, ∃ v, (l +ₗ i) ↦ v)) ∗ 
+          is_valid_loc l al) 
           ∨  
         ⌜vret = NONEV⌝)
       }}}.
   Proof. 
-    iIntros (φ) "(%res&%cap&%vs&%Hr&%Hcr & #Hal1 & Hal2 & Hisfl & Hun & %Hlen) Hphi".
-    iUnfold extend. wp_pures. wp_load. wp_load. wp_pures. 
+    iIntros (φ) "(#Hal3'&(%res&%bs'&%cap&%Hr&%Hcr&%Hbs&#Hal1&Hal2&#Hal3&Hfl&Hun))Hphi". 
+    iCombine "Hal3' Hal3" gives %[_ Heq]. simplify_eq.
+    iUnfold extend. wp_pures. wp_load. wp_load. wp_load. wp_pures. 
     destruct (decide (cap = 0)) as [Hc | Hc]. 
     { rewrite Hc. wp_pures. case_bool_decide; [|lia]. wp_pures. 
-      wp_apply ((freelist_extend_hoare al al res (al +ₗ 3) 0 0 0 0) with "[Hisfl]"); 
-      try lia; [assert ((3 + Z.of_nat 0)%Z = 3) by lia; by rewrite H0| |].
-      { iFrame "Hal1". iSplitL "Hisfl"; [done|]. iExists []. iSplit; 
-        [by rewrite array_nil|iPureIntro; by rewrite length_nil]. }
-      destruct vs; [rewrite length_nil in Hlen; lia|]. rewrite array_cons.
-      iDestruct "Hun" as "(Hun1 & Hun)".
-      iIntros "Hisfl". wp_store. wp_pures. iApply "Hphi". iSplitR "Hun1". 
-      { iExists res, 1, vs. rewrite Loc.add_assoc. iFrame. iFrame "Hal1". 
-        iSplitR; [by iPureIntro|]. iSplitR; [by iPureIntro|]. iPureIntro. 
-        simpl in Hlen. lia. }
-      iLeft. iExists (al +ₗ 3), v. iFrame. iSplitL; [done|]. iExists res, 0. auto. }
+      wp_apply ((freelist_extend_hoare al res bs' (al +ₗ 4) 0 0 0 0) with "[Hfl]"); 
+      try lia; [by rewrite Z.mul_0_l|rewrite array_nil; iFrame "Hal1 Hal3 Hfl"|].
+      rewrite Nat.sub_0_r. destruct res; [lia|]. simpl. 
+      rewrite replicate_add array_app. iDestruct "Hun" as "(Hun1 & Hun2)". 
+      iIntros "Hfl". wp_store. wp_pures. iApply "Hphi". iSplitL "Hal2 Hun2 Hfl".
+      { rewrite length_replicate Z.add_0_l. iFrame "Hal3 Hal1 Hfl". 
+        iExists 1. iFrame "Hal2". iSplitR; [by iPureIntro|]. iSplitR; 
+        [iPureIntro; lia|]. iSplitR; [by iPureIntro|]. assert (S res - 1 = res) by lia.
+        by rewrite Z.mul_0_l Z.mul_1_l Loc.add_assoc H0. }
+      iLeft. rewrite Z.mul_0_l !Z.add_0_r. iExists (al +ₗ 4). iSplitR; [done|].
+      iSplitL.
+      { iApply big_sepL_mono; [|by iApply seq_array_pointsto_eq]. iIntros. auto. }
+      iFrame "Hal3 Hal1". iExists 0. rewrite Z.mul_0_l. iPureIntro. split; [done|lia]. }
     case_bool_decide; [inv H; lia|]. wp_pures. case_bool_decide.
     { wp_pures. case_bool_decide; [inv H1; lia|]. wp_pures. 
       assert (Z.of_nat (cap - 1) = (Z.of_nat cap - 1)%Z) by lia. rewrite -H2.
-      rewrite -(take_drop (cap - 1) vs). 
-      iDestruct (array_app with "Hun") as "(Hun1 & Hun2)".
-      assert (Hlt : length (take (cap - 1) vs) = cap - 1); [rewrite length_take; lia|].
-      wp_apply (freelist_extend_hoare al al res (al +ₗ (3 + cap)) 
-      cap (cap - 1) 0 (cap - 1) with "[Hisfl Hun1]"); try lia; [done| |].
-      { iFrame "Hal1 Hisfl". rewrite Loc.add_0. iFrame. iPureIntro. by rewrite Hlt. }
-      iIntros "Hisfl". wp_store. wp_pures. iApply "Hphi". rewrite Hlt. 
-      rewrite -(take_drop 1 (drop (cap - 1) vs)). 
-      iDestruct (array_app with "Hun2") as "(Hun1 & Hun2)". iSplitR "Hun1". 
-      { iExists res, (cap + cap), (drop cap vs). rewrite Nat2Z.inj_add. 
-        iFrame. iFrame "Hal1". iSplitR; [iPureIntro; lia|]. 
-        iSplitR; [iPureIntro; lia|]. rewrite length_take length_drop Hlen.
-        iSplitL; [|iPureIntro; rewrite length_drop; lia]. 
-        assert (1 `min` (res - cap - (cap - 1)) = 1); [rewrite min_l; [done|lia]|]. 
-        rewrite H3 drop_drop 2!Loc.add_assoc -Nat2Z.inj_add. 
-        assert (cap - 1 + 1 = cap) by lia. by rewrite H4 Z.add_assoc. }
-      iLeft. rewrite Loc.add_assoc. rewrite Nat2Z.inj_sub; [|lia].
-      Search "+" "-". assert ((3 + cap + (cap - 1))%Z = (3 + cap + cap - 1)%Z) by lia. 
-      rewrite H3. iExists (al +ₗ (3 + cap + cap - 1)).
-      assert (length (drop (cap - 1) vs) > 0); [rewrite length_drop Hlen; lia|].
-      destruct (drop (cap - 1) vs); [rewrite length_nil in H4; lia|]. simpl.
-      rewrite take_0. iDestruct (array_singleton with "Hun1") as "Hun1".
-      iExists v. iFrame. iSplitR; [by iPureIntro|]. iExists res, (cap + cap - 1). 
-      iFrame "Hal1". iSplitL; [|iPureIntro; lia]. rewrite -Z.add_assoc. 
-      assert ((3 + (cap + cap) - 1)%Z = (3 + (cap + cap - 1))%Z) by lia. 
-      rewrite H5 Nat2Z.inj_sub; [|lia]. by rewrite Nat2Z.inj_add. }
+      (*split: (cap - 1) * bs' + (res - cap - (cap - 1)) * bs')*)
+      assert ((res - cap) * bs' = (cap - 1) * bs' + (res - cap - (cap - 1)) * bs') 
+      by lia. rewrite H3 replicate_add array_app. 
+      iDestruct "Hun" as "(Hun1 & Hun2)". rewrite length_replicate.
+      wp_apply (freelist_extend_hoare al res bs' (al +ₗ (4 + (cap * bs'))) cap 
+      (cap - 1) 0 (cap - 1) with "[Hfl Hun1]"); try lia; [done| |].
+      { iFrame "Hal1 Hfl Hal3". by rewrite Z.mul_0_l Loc.add_0. }
+      iIntros "Hfl". wp_store. wp_pures. iApply "Hphi".  
+      (*split: bs' of *)
+      assert (res - cap - (cap - 1) = 1 + (res - cap - cap)) by lia. rewrite H4.
+      rewrite Nat.mul_add_distr_r Nat.mul_1_l replicate_add array_app.
+      iDestruct ("Hun2") as "(Hun1 & Hun2)". iSplitR "Hun1". 
+      { rewrite -Nat2Z.inj_add. iFrame "Hal1 Hal3 Hal2 Hfl". iSplitR; [by iPureIntro|].
+        iSplitR; [iPureIntro; lia|]. iSplitR; [by iPureIntro|]. 
+        rewrite length_replicate !Loc.add_assoc. 
+        assert ((4 + cap * bs' + (((cap - 1) * bs')%nat + bs'))%Z 
+        = (4 + (cap + cap)%nat * bs')%Z) by lia.
+        assert ((res - cap - cap) * bs' = (res - (cap + cap)) * bs') by lia.
+        by rewrite H5 H6. }
+      iLeft. rewrite Loc.add_assoc. 
+      assert ((4 + (cap + cap - 1) * bs')%Z = 
+      4 + cap * bs' + ((cap - 1) * bs')%nat) by lia. rewrite H5. iExists _. 
+      iSplitR; [by iPureIntro|]. iSplitL. 
+      { iApply big_sepL_mono; [|iApply seq_array_pointsto_eq; iApply "Hun1"].
+        iIntros. iExists NONEV. 
+        assert ((4 + cap * bs' + ((cap - 1) * bs')%nat)%Z = 
+        (4 + cap * bs' + (cap - 1) * bs')%nat) by lia. by rewrite H7.  }
+      iFrame "Hal1 Hal3". iExists (cap + (cap - 1)). iPureIntro.
+      split; [|lia]. f_equal. lia. } 
     wp_pures. destruct (decide (res - cap = 0)) as [Hcr2 | Hcr2]. 
     { rewrite -Nat2Z.inj_sub; [|done]. rewrite Hcr2. wp_pures. 
-      iApply "Hphi". iSplitL; [iFrame; iFrame "Hal1"; iPureIntro; lia|].
-      iRight. by iPureIntro. }
+      iApply "Hphi". iSplitL; [|by iRight].
+      iFrame "Hal1 Hal3 Hal2 Hfl". iSplitR; [by iPureIntro|]. 
+      iSplitR; [by iPureIntro|]. iSplitR; [by iPureIntro|]. by rewrite Hcr2. }
     case_bool_decide; [inv H1; lia|]. wp_pures.
-    iPoseProof (freelist_extend_hoare al al res (al +ₗ (3 + cap)) cap 
-    (res - cap - 1) 0 (res - cap - 1)) as "H"; [lia|done|done|lia|]. 
+    (* split (res - cap - 1) * bs + bs  *)
+    assert (res - cap = (res - cap - 1) + 1) by lia. rewrite H2. 
+    rewrite Nat.mul_add_distr_r Nat.mul_1_l replicate_add array_app length_replicate. 
+    iDestruct "Hun" as "(Hun1 & Hun2)". 
+    iPoseProof (freelist_extend_hoare al res bs' (al +ₗ (4 + cap * bs')) 
+    cap (res - cap - 1) 0 (res - cap - 1)) as "H"; [lia|done|done|lia|done|]. 
     assert (Z.of_nat (res - cap - 1) = (Z.of_nat res - Z.of_nat cap - 1)%Z) by lia.
-    rewrite H2 -(take_drop (res - cap - 1) vs). 
-    iDestruct (array_app with "Hun") as "(Hun1 & Hun2)".
-    wp_apply ("H" with "[Hisfl Hun1]"). 
-    { iFrame "Hal1 Hisfl". iExists (take (res - cap - 1) vs). iSplitL "Hun1"; [
-      by rewrite Loc.add_assoc Z.add_0_r|]. iPureIntro. rewrite length_take. lia. }
-    iIntros "Hisfl". wp_store. wp_pures. iApply "Hphi".
-    rewrite -(take_drop 1 (drop (res - cap - 1) vs)). 
-    iDestruct (array_app with "Hun2") as "(Hun1 & Hun2)". iSplitR "Hun1". 
-    { iExists res, (cap + (res - cap)),  (drop (res - cap) vs). iFrame "Hal1".
-      rewrite -Nat2Z.inj_sub; [|done]. rewrite Nat2Z.inj_add. iFrame.
-      iSplitR; [done|]. iSplitR; [iPureIntro; lia|]. rewrite length_take.
-      iSplitL; [|iPureIntro; rewrite length_drop Hlen; lia].
-      rewrite Hlen. assert ((res - cap - 1) `min` (res - cap) = res - cap - 1); 
-      [rewrite min_l; [done|lia]|]. rewrite H3. rewrite length_take.
-      assert (1 `min` length (drop (res - cap - 1) vs) = 1); 
-      [rewrite length_drop Hlen min_l; [done|]; lia|]. rewrite H4. 
-      rewrite drop_drop Nat.sub_add; [|lia]. rewrite !Loc.add_assoc. 
-      assert ((Z.of_nat (res - cap - 1) + Z.of_nat 1)%Z = Z.of_nat (res - cap)) by lia.
-      by rewrite H5 Z.add_assoc. }
-    iLeft. rewrite length_take Hlen. 
-    assert ((res - cap - 1) `min` (res - cap) = res - cap - 1); 
-    [rewrite min_l; [done|lia]|]. rewrite H3. 
-    assert (length (drop (res - cap - 1) vs) > 0); [rewrite length_drop Hlen; lia|].
-    destruct (drop (res - cap - 1) vs); [rewrite length_nil in H4; lia|]. simpl. 
-    rewrite take_0 array_singleton 2!Loc.add_assoc -Nat2Z.inj_sub; [|done].
-    assert ((3 + cap + Z.of_nat (res - cap - 1))%Z = 
-    (3 + cap + Z.of_nat (res - cap) - 1)%Z) by lia. 
-    rewrite H5. iExists (al +ₗ (3 + cap + (res - cap)%nat - 1)), v. iSplitR; 
-    [by iPureIntro|]. iFrame. iExists res, (cap + (res - cap)%nat - 1). iFrame "Hal1".
-    iSplitR; [iPureIntro|iPureIntro; lia]. 
-    rewrite -Z.add_assoc -Nat2Z.inj_add -Z.add_sub_assoc Nat2Z.inj_sub; [done|lia].
+    rewrite H3. wp_apply ("H" with "[Hfl Hun1]"). 
+    { rewrite Loc.add_assoc Z.mul_0_l Z.add_0_r. iFrame "Hfl Hun1 Hal1 Hal3". }
+    iIntros "Hfl". wp_store. wp_pures. iApply "Hphi". 
+    (* split bs' of*) 
+    iSplitL "Hfl Hal2". 
+    { rewrite -Nat2Z.inj_sub; [|done]. rewrite -Nat2Z.inj_add. 
+      iFrame "Hal1 Hal2 Hal3 Hfl". iSplitR; [by iPureIntro|]. iSplitR; 
+      [iPureIntro; lia|]. iSplitR; [by iPureIntro|].
+      assert (res - (cap + (res - cap)) = 0) by lia. rewrite H4 Nat.mul_0_l.
+      simpl. by rewrite array_nil. }
+    iLeft. rewrite !Loc.add_assoc. 
+    assert ((4 + cap * bs' + ((res - cap - 1) * bs')%nat)%Z 
+    = (4 + (cap + (res - cap) - 1) * bs')%Z) by lia. rewrite H4. 
+    iExists _. iSplitR; [by iPureIntro|]. iSplitL.
+    { iApply big_sepL_mono; [|by iApply seq_array_pointsto_eq]. iIntros. auto. }
+    iFrame "Hal1 Hal3". iExists (cap + (res - cap) - 1). iSplitR; [|iPureIntro; lia].
+    Set Printing Coercions. rewrite -Nat2Z.inj_sub; [|lia]. rewrite -Nat2Z.inj_add.
+    assert ((Z.of_nat (cap + (res - cap)) - 1)%Z 
+    = (Z.of_nat (cap + (res - cap) - 1))%Z) by lia. by rewrite H5. 
   Qed.
 
-  Lemma alloc_hoare al :
-    {{{ is_allocator al }}}
+  (*TODO(Ben): bs is in the way*)
+  Lemma alloc_hoare al bs :
+    {{{ (al +ₗ 3) ↦□ #bs ∗ is_allocator al }}}
       alloc #al
     {{{ vret, RET vret; 
       is_allocator al ∗
-      ((∃ l v, ⌜vret = SOMEV #l⌝ ∗ l ↦ v ∗ is_valid_loc l al)
+      ((∃ l, ⌜vret = SOMEV #l⌝ ∗ ([∗ list] i ∈ seq 0 bs, ∃ v, (l +ₗ i) ↦ v) ∗ 
+        is_valid_loc l al)
         ∨ 
       ⌜vret = NONEV⌝)
     }}}.
   Proof.
-    iIntros (φ) "(%res&%cap&%vs&%Hr& %Hcr & Hal1 & Hal2 & Hisfl & Hun & %Hlen) Hphi". 
-    iUnfold alloc. wp_pures. wp_apply (freelist_pop_hoare with "Hisfl"). 
-    iIntros (v) "(Hisfl & [->|(%l & %v' & -> & Hl & #Hlv)])".
-    { wp_pures. wp_apply (extend_hoare with "[Hal1 Hal2 Hun Hisfl]"); 
-      [iFrame; iPureIntro; lia|]. iIntros (v) "(Hal & [(%l & %v' & -> & Hisfl)| ->])"; 
-      iApply "Hphi"; iSplitL "Hal"; try done; [iLeft; by iFrame|by iRight]. }
-    wp_pures. iApply "Hphi". iSplitR "Hl"; [iFrame; iPureIntro; lia|].
-    iLeft. iFrame. iSplitR; [by iPureIntro|done]. 
+    iIntros (φ) "(#Hal3'&(%res&%bs'&%cap&%Hr&%Hcr&%Hbs&#Hal1&Hal2&#Hal3&Hfl&Hun))Hphi". 
+    iCombine "Hal3' Hal3" gives %[_ Heq]. simplify_eq.
+    iUnfold alloc. wp_pures. 
+    wp_apply (freelist_pop_hoare with "[Hfl]"); [iFrame "Hfl Hal3"|].
+    iIntros (v) "(Hfl & [-> | (%l & -> & Hlbs & Hlv)])"; wp_pures.
+    { wp_apply (extend_hoare with "[Hal2 Hun Hfl]"); 
+      [iFrame "Hal1 Hal2 Hal3 Hfl Hun"; iPureIntro; lia|]. 
+      iIntros (v) "(Hal & [(%l & -> & Hlbs & Hlv) | ->])"; iApply "Hphi"; 
+      [iFrame; iLeft; iFrame; auto|iFrame; by iRight]. } 
+    iApply "Hphi". iFrame. iSplitR; [iFrame "Hal1 Hal3"; iPureIntro; lia|].
+    iLeft. iFrame "Hlbs". by iSplitR. 
   Qed.
 
 End Hoare.
